add typing for stlc/autosubst2

stlc/autosubst2/def_typing.v
@@ -1,3 +1,28 @@
-Require Import stlc.autosubst2.def.
+Require Import stlc.autosubst2.def_as2.
+
+Require Import List.
 
 (* https://github.com/yiyunliu/autosubst-stlc/blob/master/typing.v *)
+
+Definition ctx := list typ.
+
+Inductive lookup {T} : nat -> list T -> T -> Prop :=
+| here A Γ : lookup 0 (A :: Γ) A
+| there n Γ A B : lookup n Γ A -> lookup (S n) (cons B Γ) A.
+
+Reserved Notation "Γ ⊢ t : A" 
+  (at level 50, t at next level, no associativity).
+Inductive typing : ctx -> exp -> typ -> Prop :=
+| typing_unit : forall (Γ : ctx),
+  Γ ⊢ exp_unit : typ_unit
+| typing_var : forall (Γ : ctx) (i : nat) (A : typ),
+  lookup i Γ A ->
+  Γ ⊢ (exp_var i) : A
+| typing_abs : forall (Γ : ctx) (A B : typ) (t : exp),
+  (A :: Γ) ⊢ t : B ->
+  Γ ⊢ (exp_abs t) : (typ_arr A B)
+| typing_app : forall (Γ : ctx) (s t : exp) (A B : typ),
+  Γ ⊢ s : (typ_arr A B) ->
+  Γ ⊢ t : A ->
+  Γ ⊢ (exp_app s t) : B
+where "Γ ⊢ t : A" := (typing Γ t A).
