stlc/autosubst2/prop_typing.v
@@ -1,0 +1,26 @@
+Require Import stlc.autosubst2.prop_as_core.
+Require Import stlc.autosubst2.prop_as_unscoped.
+Require Import stlc.autosubst2.def_as2.
+Require Import stlc.autosubst2.def_typing.
+
+Definition ctx_var_rename {T} ζ Γ Δ :=
+  forall i (A : T), lookup i Γ A -> lookup (ζ i) Δ A.
+
+Import SubstNotations.
+Import UnscopedNotations.
+
+Hint Constructors lookup typing : core.
+
+Theorem typing_rename Γ t A : 
+  Γ ⊢ t : A ->
+  forall Δ ζ,
+    ctx_var_rename ζ Γ Δ ->
+    Δ ⊢ t ⟨ζ⟩ : A.
+Proof.
+  intros H. induction H; intros; asimpl; eauto.
+  - apply typing_abs. 
+    eapply IHtyping; eauto.
+    unfold ctx_var_rename in *. intros.
+    inversion H1; subst; asimpl; eauto.
+    econstructor. eauto.
+Qed.
